Efficient refinement of the NumOrders query in the Bookstore example (!)
(The file needs a serious cleanup, but some of the code in here was
never committed).

examples/Bookstore.experimental.v
@@ -1,6 +1,9 @@
 Section BookStoreExamples.
   Require Import QueryStructureNotations.
   Require Import ListImplementation.
+  Require Import AdditionalLemmas AdditionalMorphisms.
+
+  Unset Implicit Arguments.
 
   (* Our bookstore has two relations (tables):
      - The [Books] relation contains the books in the
@@ -19,26 +22,28 @@ Section BookStoreExamples.
      constraint.
    *)
 
-  Check (schema <"Author" :: string,
-         "Title" :: string,
-         "ISBN" :: nat>
-         where attributes ["Title"; "Author"] depend on ["ISBN"]).
+  Definition sBOOKS := "Books".
+  Definition sAUTHOR := "Authors".
+  Definition sTITLE := "Title".
+  Definition sISBN := "ISBN".
+  Definition sORDERS := "Orders".
+  Definition sDATE := "Date".
 
   Definition BookStoreSchema :=
     Query Structure Schema
-      [ relation "Books" has
-                schema <"Author" :: string,
-                        "Title" :: string,
-                        "ISBN" :: nat>
-                        where attributes ["Title"; "Author"] depend on ["ISBN"];
-        relation "Orders" has
-                schema <"ISBN" :: nat,
-                        "Date" :: nat> ]
-      enforcing [attribute "ISBN" of "Orders" references "Books"].
+      [ relation sBOOKS has
+                schema <sAUTHOR :: string,
+                        sTITLE :: string,
+                        sISBN :: nat>
+                where attributes [sTITLE; sAUTHOR] depend on [sISBN];
+        relation sORDERS has
+                schema <sISBN :: nat,
+                        sDATE :: nat> ]
+      enforcing [attribute sISBN of sORDERS references sBOOKS].
 
   (* Aliases for the tuples contained in Books and Orders, respectively. *)
-  Definition Book := TupleDef BookStoreSchema "Books".
-  Definition Order := TupleDef BookStoreSchema "Orders".
+  Definition Book := TupleDef BookStoreSchema sBOOKS.
+  Definition Order := TupleDef BookStoreSchema sORDERS.
 
   (* Our bookstore has two mutators:
      - [PlaceOrder] : Place an order into the 'Orders' table
@@ -63,31 +68,66 @@ Section BookStoreExamples.
       const "InitBookstore" (_ : unit) : rep := empty,
 
       update "PlaceOrder" ( o : Order ) : unit :=
-          Insert o into "Orders",
+          Insert o into sORDERS,
 
       update "AddBook" ( b : Book ) : unit :=
-          Insert b into "Books" ,
+          Insert b into sBOOKS ,
 
       query "GetTitles" ( author : string ) : list string :=
-        For (b in "Books")
-        Where (author = b!"Author")
-        Return (b!"Title"),
+        For (b in sBOOKS)
+        Where (author = b!sAUTHOR)
+        Return (b!sTITLE),
 
        query "NumOrders" ( author : string ) : nat :=
-          Count (For (o in "Orders") (b in "Books")
-                 Where (author = b!"Author")
-                 Where (b!"ISBN" = o!"ISBN")
-                 Return o!"ISBN")
+          Count (For (o in sORDERS) (b in sBOOKS)
+                 Where (author = b!sAUTHOR)
+                 Where (b!sISBN = o!sISBN)
+                 Return o!sISBN)
   }.
 
-  Require Import BagsOfTuples.
+  Require Import BagsOfTuples Bool.
+
+  (* (* TODO *)
+  Eval compute in 
+      (
+        let relation_key := 
+            (fun (x : BoundedIndex (map relName (qschemaSchemas BookStoreSchema))) => x)
+              {| bindex := sBOOKS; indexb := _ |} in
+        let attribute_key := 
+            (fun (x :  Attributes (GetNRelSchemaHeading (qschemaSchemas BookStoreSchema) relation_key)) => x)
+              {| bindex := sISBN; indexb := _ |} in
+        attribute_key
+      ).
+   *)
+  
+  Notation "qs_schema / rel_index" := (GetRelationKey qs_schema rel_index) (at level 40, left associativity).
+  Notation "rel_key // attr_index" := (GetAttributeKey rel_key attr_index) (at level 50).
+
+  Definition Books := BookStoreSchema/sBOOKS. 
+  Definition Orders := BookStoreSchema/sORDERS.
+  Definition BookSchema := QSGetNRelSchemaHeading BookStoreSchema Books.
+  Definition OrderSchema := QSGetNRelSchemaHeading BookStoreSchema Orders.
+
+  Definition BookStorage : @BagPlusBagProof Book.
+    mkIndex BookSchema [ Books//sAUTHOR; Books//sISBN ].
+  Defined.
+
+  Definition OrderStorage : @BagPlusBagProof Order.
+    mkIndex OrderSchema [ Orders//sISBN ].
+  Defined.
+
+  Definition TBookStorage := BagType BookStorage.
+  Definition TOrderStorage := BagType OrderStorage.
 
   Definition BookStoreListImpl_AbsR
              (or : UnConstrQueryStructure BookStoreSchema)
-             (nr : list Book * list Order) : Prop :=
-    or ! "Books" ≃ benumerate (fst nr) /\ or ! "Orders" ≃ benumerate (snd nr).
+             (nr : TBookStorage * TOrderStorage) : Prop :=
+    or ! sBOOKS ≃ benumerate (fst nr) /\ or ! sORDERS ≃ benumerate (snd nr).
 
   Opaque Query_For.
+  Opaque benumerate bfind_matcher bfind benumerate. (* TODO *)
+
+  (* TODO: How to do the instantiations automatically? *)
 
   Definition BookStore :
     Sharpened BookStoreSpec.
@@ -98,189 +138,721 @@ Section BookStoreExamples.
       of a client of a sharpened ADT the invariants will still hold,
       since ADT refinement preserves the simulation relation. *)
 
-    start honing QueryStructure.
+    match goal with
+        |- context [@BuildADT (QueryStructure ?Rep) _ _ _ _] =>
+        hone representation using (@DropQSConstraints_AbsR Rep)
+    end.
+    
+    drop constraints from insert "PlaceOrder".
+    drop constraints from insert "AddBook".
+    drop constraints from query "GetTitles".
+    drop constraints from query "NumOrders".
+
+    (*TODO: start honing QueryStructure.*)
 
     hone representation using BookStoreListImpl_AbsR.
 
-    hone method "PlaceOrder".
-    {
-      setoid_rewrite refineEquiv_pick_ex_computes_to_bind_and.
-      rewrite refine_pick_val with (A := nat) (a := length (snd r_n)).
+    hone constructor "InitBookstore". {
+       unfold BookStoreListImpl_AbsR.
+
+      repeat setoid_rewrite refineEquiv_pick_ex_computes_to_and;
+      repeat setoid_rewrite refineEquiv_pick_eq';
       simplify with monad laws.
-      setoid_rewrite refineEquiv_split_ex.
-      setoid_rewrite refineEquiv_pick_computes_to_and.
-      simplify with monad laws.
-      (* TODO: remove this etransitivity, apply step. *)
-      etransitivity.
-      apply refine_bind.
-      eapply (@refine_foreign_key_check
-                 _
-                 _ (fst r_n)
-      (fun tup2 : Tuple => n ``("ISBN") = tup2 ``("ISBN"))).
-      destruct H; eauto.
-      unfold pointwise_relation; intros; higher_order_1_reflexivity.
-      (* END TODO*)
-      simplify with monad laws.
-      unfold If_Then_Else; rewrite refine_if_bool_eta.
-      simplify with monad laws.
-      rewrite refine_pick_eq_ex_bind; unfold BookStoreListImpl_AbsR in *.
-      split_and; simpl;
-      rewrite refineEquiv_pick_pair_pair;
+
+      rewrite (refine_pick_val' (bempty, bempty)) by (intuition; apply bempty_correct_DB).
+      subst_body; higher_order_1_reflexivity. 
+    }
+
+    Notation "?[ A ]" := (if A then true else false) (at level 50).
+
+    hone method "NumOrders". {
+      unfold BookStoreListImpl_AbsR in H; split_and.
+      
+      setoid_rewrite refineEquiv_pick_ex_computes_to_and;
+      setoid_rewrite refineEquiv_pick_pair;
       setoid_rewrite refineEquiv_pick_eq';
-      simplify with monad laws; simpl.
-      Split Constraint Checks.
-      (* TODO move this back to a tactic *)
+      simplify with monad laws; cbv beta;
+      simpl.
+ 
+      (* Step 1: Move to a concrete representation *)
+
+      rewrite refine_List_Query_In by eassumption.
+      rewrite refine_Join_List_Query_In by eassumption.
+      rewrite refine_List_Query_In_Where; instantiate (1 := _).
+      rewrite refine_List_Query_In_Where; instantiate (1 := _).
+      rewrite refine_List_For_Query_In_Return_Permutation.
+      simpl.
+
+      (* Step 2: Make it more efficient *)
+
+      rewrite (filter_join_snd (fun (a: Book) => ?[string_dec n (a!sAUTHOR)])).     
+      rewrite (filter_by_equiv _ (bfind_matcher (Bag := BagProof BookStorage) (Some n, (None, [])))) 
+        by prove_observational_eq.
+
+      setoid_rewrite swap_joins; trickle_swap; simpl.
+
+      setoid_rewrite filter_join_lists; simpl.
+      setoid_rewrite (filter_by_equiv_meta
+                 (fun (x: Book) (y : Order) => ?[eq_nat_dec x!sISBN y!sISBN]) 
+                 (fun (x: Book) => bfind_matcher (Bag := BagProof OrderStorage) (Some x!sISBN, [])) _).
+
+      setoid_rewrite map_flat_map.      
+      setoid_rewrite map_map; simpl.
+      
+      setoid_rewrite (bfind_correct _).
+      setoid_rewrite refine_Permutation_Reflexivity.
+      simplify with monad laws.
+      
+      (* Step 3: Finish honing *)
+      unfold BookStoreListImpl_AbsR.
+      rewrite refine_pick_val by eauto.
+      simplify with monad laws.
+      
+      (* Step 4: Final tweaks *)
+      setoid_rewrite length_flat_map.
+      setoid_rewrite map_length.
+
+      (* Step 5: All done *)
+      finish honing.
+    }
+
+    hone method "GetTitles". {
+      unfold BookStoreListImpl_AbsR in H; split_and.
+      
+      setoid_rewrite refineEquiv_pick_ex_computes_to_and;
+      setoid_rewrite refineEquiv_pick_pair;
+      setoid_rewrite refineEquiv_pick_eq';
+      simplify with monad laws; cbv beta;
+      simpl.
+ 
+      rewrite refine_List_Query_In by eassumption.
+      setoid_rewrite refine_List_Query_In_Where.
+      rewrite refine_List_For_Query_In_Return_Permutation.
+
+      rewrite (filter_by_equiv _ (bfind_matcher (Bag := BagProof BookStorage) (Some n, (None, [])))) by
+          prove_observational_eq.
+      
+      setoid_rewrite (bfind_correct _).
+      setoid_rewrite refine_Permutation_Reflexivity.
+      simplify with monad laws.
+
+      unfold BookStoreListImpl_AbsR.
+      rewrite refine_pick_val by eauto. 
+      simplify with monad laws.
+      finish honing.
+    }
+
+      pose proof (fun f => filter_by_equiv f (bfind_matcher (Bag := BagProof BookStorage) (Some n, (None, []))) _ (Join_Lists (benumerate (snd r_n))
+                          (benumerate (fst r_n)))). by
+          prove_observational_eq.
+      
+      setoid_rewrite refineEquiv_pick_pair_pair.
+      setoid_rewrite refineEquiv_pick_eq'.
+      simplify with monad laws.
+      rewrite refine_pick_val by eassumption.
+      simplify with monad laws.
+      rewrite refine_pick_val by eassumption.
+      simplify with monad laws.
+      finish honing.
+
+      rewrite refine_List_Query_In by eassumption.
+      setoid_rewrite refine_List_Query_In. by eassumption.
+      setoid_rewrite refine_List_Query_In_Where.
+      rewrite refine_List_For_Query_In_Return_Permutation.
+
+      rewrite (filter_by_equiv _ (bfind_matcher (Bag := BagProof BookStorage) (Some n, (None, [])))) by
+          prove_observational_eq.
+      
+      setoid_rewrite (bfind_correct _).
+      setoid_rewrite refine_Permutation_Reflexivity.
+      simplify with monad laws.
+
+      unfold BookStoreListImpl_AbsR.
+      rewrite refine_pick_val by eauto. 
+      simplify with monad laws.
+      finish honing.
+
+    Class IsDecidableBinaryPredicate {A B: Type} (predicate: A -> B -> Prop) :=
+      { 
+        bool_predicate : A -> B -> bool; 
+        is_decidable : 
+          forall a b, 
+            bool_predicate a b = true <-> predicate a b 
+      }.
+
+    Check @bool_predicate.
+    Lemma CrossProduct :
+      forall {TReturn TRecord1 TRecord2: Type},
+      forall (table1: list TRecord1) (table2: list TRecord2) query_body,
+      forall predicate (proof: IsDecidableBinaryPredicate predicate),
+        Equivalent_Ensembles
+          (fun retval : TReturn =>
+             exists joined_records : TRecord1 * TRecord2,
+               List.In joined_records (Join_Lists table1 table2)
+               /\ Where (predicate (fst joined_records) (snd joined_records)) 
+                        (query_body (fst joined_records) (snd joined_records)) retval)
+          (fun retval : TReturn =>
+             exists joined_records : TRecord1 * TRecord2,
+               List.In joined_records (Join_Lists table1 (List.filter (fun record2 => bool_predicate (fst joined_records) record2) table2))
+               /\ (query_body (fst joined_records) (snd joined_records) retval)).
+    Proof.
+      unfold Equivalent_Ensembles, Query_Where; intros.
+      apply Morphisms_Prop.ex_iff_morphism.
+      unfold pointwise_relation.
+      intros (rec1 & rec2); simpl.
+      unfold Join_Lists; simpl.
+
+      rewrite <- and_assoc.
+      apply and_iff_compat_r.
+      setoid_rewrite flat_map_flatten.
+      setoid_rewrite in_flatten_iff.
+
+      split; intro H;
+      [ destruct H as ( [ seq (rec12_in_seq & seq_in_map) ] & pred12) |
+        destruct H as [ seq (rec12_in_seq & seq_in_map) ] ];
+      rewrite in_map_iff in seq_in_map;
+      destruct seq_in_map as [ rec1' (eq_ & in1) ]; subst;
+      rewrite in_map_iff in rec12_in_seq;
+      destruct rec12_in_seq as [ rec2' (eq_ & in2) ]; inversion eq_; subst; clear eq_.
+      {
+        eexists; split;
+        [ | rewrite in_map_iff; eexists]; eauto.
+        rewrite in_map_iff; eexists; split; eauto.
+        rewrite filter_In; split; try apply is_decidable; eauto.
+      } {
+        rewrite filter_In in in2.
+        destruct in2 as (in2 & pred_satisfied).
+        eexists; [ eexists; split; [ | rewrite in_map_iff ] | apply is_decidable; assumption ]; eauto.
+        rewrite in_map_iff; eexists; split; eauto.
+      }
+    Qed.
+
+    assert (IsDecidableBinaryPredicate
+              (fun (rec1 : Book) (rec2 : Order) => rec1!sISBN = rec2!sISBN)).
+    econstructor.
+    intros.
+    rewrite <- beq_nat_true_iff.
+    instantiate (1 := fun a b => _ a!sISBN b!sISBN).
+    cbv beta.
+    reflexivity. (* congruence here crashes *)
+
+    Lemma CrossProduct' :
+      forall {TReturn TRecord1 TRecord2: Type},
+      forall (table1: list TRecord1) (table2: list TRecord2) query_body,
+      forall bpredicate,
+        Equivalent_Ensembles
+          (fun retval : TReturn =>
+             exists joined_records : TRecord1 * TRecord2,
+               List.In joined_records 
+                       (Join_Lists 
+                          table1 
+                          (List.filter 
+                             (fun record2 => bpredicate (fst joined_records) record2) table2))
+               /\ (query_body (fst joined_records) (snd joined_records) retval))
+          (fun retval : TReturn =>
+             exists joined_records : TRecord1 * TRecord2,
+               List.In joined_records 
+                       (flat_map
+                          (fun a =>
+                             map (fun b => (a, b))
+                                 (filter
+                                    (fun b => bpredicate a b) table2))
+                          table1)
+               /\ (query_body (fst joined_records) (snd joined_records) retval)).
+    Proof.
+      unfold Equivalent_Ensembles, Join_Lists.
+      setoid_rewrite flat_map_flatten.
+      intros.
+      
+      split; intro H;
+      destruct H as [ rec12 (in_join & qbody) ];
+
+      rewrite in_flatten_iff in in_join;
+      destruct in_join as [ seq (in_seq & seq_in_map) ];
+      rewrite in_map_iff in seq_in_map;
+      destruct seq_in_map as [ rec1' (seq_eq & in1) ];
+      subst seq;
+      rewrite in_map_iff in in_seq;
+      destruct in_seq as [ rec2' (eq_12_1'2' & in_filter) ];
+      rewrite <- eq_12_1'2' in *;
+      rewrite filter_In in in_filter;
+      destruct in_filter as (in2 & pred_satisfied);
+      
+      eexists;
+      rewrite in_flatten_iff;
+      (split;
+       [ eexists; split; [ | rewrite in_map_iff; eexists ] | eassumption ]; eauto;
+       rewrite in_map_iff; eexists; split; eauto; rewrite filter_In; split; tauto
+      ).
+    Qed.
+
+
+      Add Parametric Morphism {A B: Type} (seq: list B) :
+        (fun pred a => List.filter (fun b => pred a b) seq)
+          with signature (pointwise2_relation A B (@eq bool) ==> (pointwise_relation _ (@eq (list B))))
+            as filter_morphism_2.
+      Proof.
+        unfold pointwise_relation, pointwise2_relation.
+        intros.
+        apply filter_eq_morphism; unfold pointwise_relation; trivial.
+      Qed.
+
+    Set Printing All.
+    Show.
+    
+    (* TODO: Look into this 
+    Typeclasses Opaque BoundedString Attribute. *)
+
+    hone method "NumOrders". {
+      unfold equivalence, UnConstrRelationAbsR, EnsembleListEquivalence_AbsR in H.
+      destruct H.
+
+      setoid_rewrite refineEquiv_pick_ex_computes_to_and;
+      setoid_rewrite refineEquiv_pick_pair;
+      setoid_rewrite refineEquiv_pick_eq';
+      simplify with monad laws; cbv beta;
+      simpl.
+
+      rewrite Equivalent_UnConstr_In_EnsembleListEquivalence by eassumption.
+      setoid_rewrite Equivalent_List_In_Where.
+
+      rewrite (filter_eq_restricted_morphism _ (y := bfind_matcher (Bag := BagProof BookStorage) (Some n, (None, [])))) by (clear; admit).
+
+      rewrite Equivalent_Join_Lists by eassumption.
+
+      setoid_rewrite (@CrossProduct nat Book Order _ _ (fun b1 b2 a => Return b2!sISBN a) (fun (rec1: Book) (rec2: Order) => rec1!sISBN = rec2!sISBN) _).
+
+      setoid_rewrite (@CrossProduct' nat Book Order _ _ (fun b1 b2 a => Return b2!sISBN a)).
+
+      setoid_rewrite flat_map_flatten.
+      setoid_rewrite (bfind_correct _). 
+      setoid_rewrite <- flat_map_flatten.
+
+      pose proof filter_morphism_2.
+      specialize (fun pred => H2 _ _ (benumerate (snd r_n)) (fun (a: Book) (b : Order) => pred a b)  (fun (a: Book) (b: Order) => bfind_matcher (Bag := BagProof OrderStorage) (Some a!sISBN, []) b) ).
+      unfold pointwise_relation, pointwise2_relation in H2.
+
+      assert (forall (a : Book) (a' : Order),
+                @bool_predicate _ _ _ X a a' = bfind_matcher (Bag := BagProof OrderStorage) (Some a!sISBN, []) a').
+      clear; admit.
+
+      specialize (H2 (@bool_predicate _ _ _ X) H3).
+      setoid_rewrite H2. 
+
+      (* More morphism needed
+      setoid_rewrite flat_map_flatten.
+      setoid_rewrite (bfind_correct _). 
+      setoid_rewrite <- flat_map_flatten.
+       *) 
+      Require Import Permutation.
+      assert (forall a: Book,
+          Permutation
+                            (map (fun b : Order => (a, b))
+                              (filter
+                                 (fun b : Order =>
+                                  bfind_matcher (Bag:=BagProof OrderStorage)  (Some a!sISBN, []) b)
+                                 (benumerate (Bag:=BagProof OrderStorage) (snd r_n))))
+          nil) by (clear; admit).
+
+      assert (
+          Permutation 
+            (flatten (map
+               (fun a : Book =>
+                  map (fun b : Order => (a, b))
+                      (filter
+                         (fun b : Order =>
+                            bfind_matcher (Bag:=BagProof OrderStorage)  (Some a!sISBN, []) b)
+                         (benumerate (Bag:=BagProof OrderStorage) (snd r_n))))
+               (bfind (fst r_n) (Some n, (None, [])))))
+            (flatten (map
+               (fun a : Book => [])
+               (bfind (fst r_n) (Bag:=BagProof BookStorage) (Some n, (None, [])))))).
+
+      Check flatten_map_permutation_permutation_permutation_morphism.
+
+      Unset Ltac Debug.
+      setoid_rewrite H4.
+      
+      apply flatten_map_permutation_permutation_permutation_morphism; eauto.
+
+      
+
+      
+            
+      setoid_rewrite H4.
+
+
+      assert ( forall bag (search_term : SearchTermType OrderStorage),
+       Permutation (filter (bfind_matcher (Bag:=BagProof OrderStorage) search_term) (benumerate (Bag:=BagProof OrderStorage) bag))
+         (bfind (Bag:=BagProof OrderStorage) bag search_term)).
+      clear; admit.
+
+
+      Require Import SetoidList.
+
+      Add Parametric Morphism {A B: Type} (seq: list A) :
+        (fun comp => List.map comp seq)
+          with signature (pointwise_relation A (@eq B) ==> (@eq (list B)))
+            as restricted_map_morphism.
+      Proof.
+        intros.
+        setoid_rewrite H; trivial.
+      Qed.
+
+      setoid_rewrite H5.
+
+      Check (bfind_correct (Bag:= BagProof (OrderStorage)) _).
+setoid_rewrite (bfind_correct _).
+      intros.
+
       etransitivity.
-      apply refine_bind.
-      match goal with
-          |- context
-               [{a | EnsembleIndexedListEquivalence
-                       ((@UpdateUnConstrRelation ?QSSchema ?c ?Ridx
-                                                (EnsembleInsert ?n (?c!?R)))!?R')%QueryImpl a}%comp] =>
-          let H := fresh in
-          generalize ((@ImplementListInsert_neq QSSchema
-                                                {| bindex := R' |}
-                                                {| bindex := R |} n c)) as H; intros; setoid_rewrite H
-      end; try reflexivity; try eassumption.
-      subst_body; congruence.
+      
+
+      setoid_rewrite H2.
+      setoid_rewrite filter_morphism_2.
+
+
+      rewrite (filter_morphism).
+      
+Require Import Setoid.
+
+Typeclasses eauto := debug. (* 5 *)
+
+Goal (forall {A B} (P Q: B -> A -> Prop) (R: B -> Prop), (forall x a, P x a <-> Q x a) -> (refine (For (fun a => exists b, R b /\ P b a)) (For (fun a => exists b, R b /\ Q b a)))).
+intros.
+setoid_rewrite H.
+reflexivity.
+Qed.
+
+
+Show.
+
+      rewrite Equivalent_UnConstr_In_EnsembleListEquivalence by eassumption.
+      rewrite Equivalent_List_In_Where.
+
+      unfold dec.
+
+      Show Existentials.
+
+      assert (DecideableEnsemble (fun b : Book => n = b!sAUTHOR)).
+      eauto with typeclass_instances.
+      
+      pose (decider := fun (b: Book) (c: Order) => if eq_nat_dec b!sISBN c!sISBN then true else false).
+      assert (forall (b: Book) (c: Order), decider b c = true <-> b!sISBN = c!sISBN) 
+        as P_dec
+          by (clear; unfold decider; intros; destruct (eq_nat_dec _ _); intuition).
+
+      Lemma Equivalent_List_In_Where' :
+        forall (A B C: Type) (l : list C) (P : B -> C -> Prop)
+               (bod : B -> C -> Ensemble A) decider (P_dec : forall b c, decider b c = true <-> P b c),
+          forall a b c,
+            (List.In c l /\ Where (P b c) (bod b c) a) <->
+            (List.In c (filter (decider b) l) /\ (bod b c) a).
+        unfold Query_Where; intros;
+        rewrite filter_In; split; intuition;
+        apply P_dec; intuition.
+      Qed.
+
+      assert (refine For (fun a : nat =>
+                          exists b : Book,
+                            List.In b
+                                    (filter
+                                       (let (dec, _) :=
+                                            DecideableEnsemble_EqDec Astring_eq
+                                                                     (fun _ : Tuple => n)
+                                                                     (fun a0 : Book => a0!sAUTHOR) in
+                                        dec) (benumerate (fst r_n))) /\
+                            UnConstrQuery_In c Orders
+                                             (fun tup : Tuple =>
+                                                Where (b!sISBN = tup!sISBN)
+                                                      Return tup!sISBN ) a)
+                     For (fun a : nat =>
+                            exists b : Book,
+                              List.In b
+                                      (filter
+                                         (let (dec, _) :=
+                                              DecideableEnsemble_EqDec Astring_eq
+                                                                       (fun _ : TupleDef BookStoreSchema sBOOKS => n)
+                                                                       (fun a0 : Book => a0!sAUTHOR) in
+                                          dec) (benumerate (fst r_n))) /\
+                              (exists tup : Order,
+                                 List.In tup (filter (decider b) (benumerate (snd r_n))) /\
+                                 Return tup!sISBN a))).
+      clear H0.
+
+      (*setoid_rewrite Equivalent_UnConstr_In_EnsembleListEquivalence.*)
+
+
+      About Equivalent_UnConstr_In_EnsembleListEquivalence.
+      pose proof (fun bod => @Equivalent_UnConstr_In_EnsembleListEquivalence nat _ c Orders (benumerate (snd r_n)) bod) as equiv. 
+      unfold Equivalent_Ensembles in equiv.
+      setoid_rewrite (fun bod => equiv bod _).
+
+      Hint Unfold pointwise_relation Equivalent_Ensembles.
+      setoid_rewrite Equivalent_UnConstr_In_EnsembleListEquivalence.
+
+ 
+
+      etransitivity.
+
+      apply refine_Query_For.
       unfold pointwise_relation; intros.
-      subst_strings; setoid_rewrite (@ImplementListInsert_eq); eauto.
-      simplify with monad laws.
-      higher_order_1_reflexivity.
-      simplify with monad laws.
-      reflexivity.
-      rewrite refine_pick_val; eauto.
-      simplify with monad laws.
-      rewrite refine_pick_val; eauto.
-      simplify with monad laws.
-      reflexivity.
+      apply exists_iff.
+      unfold pointwise_relation; intros.
+
+      apply and_iff_compat_l.
+
+      apply Equivalent_UnConstr_In_EnsembleListEquivalence.
+      eassumption.
+
+       *)
+
+      apply exists_iff.
+      unfold pointwise_relation; intros.
+
+      pose proof (fun P bod decider P_dec => @Equivalent_List_In_Where' nat Book Order (benumerate (snd r_n)) P bod decider P_dec a a0 a1) as specialized.
+
+      apply (specialized (fun book order => book!sISBN = order!sISBN) (fun book order => Return order!sISBN)).
+      assumption.
+eauto.
+      
+      setoid_rewrite equiv.
+
+      Lemma ugh : forall (A B B': Prop), (B <-> B') -> (A /\ B <-> A /\ B').
+        intros. tauto.
+      apply exi
+
+
+      setoid_rewrite equiv.
+
+      pose proof (fun a b c P bod decider P_dec => @Equivalent_List_In_Where' nat Book Order (benumerate (snd r_n)) P bod decider P_dec a b c) as where''.
+
+      pose proof (fun a b c bod => where'' a b c _ bod decider P_dec) as where'''.
+
+      assert (forall (a: nat) (b: Book), 
+                (exists tup : Tuple,
+                   List.In tup (benumerate (snd r_n)) /\
+                   Where (b!sISBN = tup!sISBN)
+                         Return tup!sISBN  a) <->
+                (exists tup : Order, 
+                   List.In tup (filter (decider b) (benumerate (snd r_n))) 
+                   /\ Return tup!sISBN a)) as where''''.
       intros.
-      destruct H as [_ [l l']].
-      generalize (l _ H1).
-      unfold not; intros.
-      eapply lt_irrefl.
-      destruct tup; simpl in *; subst.
-      eapply H.
-    }
-
-    hone method "AddBook".
-    {
-      setoid_rewrite refineEquiv_pick_ex_computes_to_bind_and.
-      rewrite refine_pick_val with (A := nat) (a := length (fst r_n)).
-      simplify with monad laws.
-      setoid_rewrite refineEquiv_split_ex.
-      setoid_rewrite refineEquiv_pick_computes_to_and.
-      simplify with monad laws.
-      rewrite refine_tupleAgree_refl_True;
-        simplify with monad laws.
-      (* Again, to tactics *)
-      repeat match goal with
-          |- context [
-                 forall tup' : @IndexedTuple ?h,
-                   (?qs ! ?R )%QueryImpl tup' ->
-                   tupleAgree ?n (indexedTuple tup') ?attrlist2%SchemaConstraints ->
-                   tupleAgree ?n (indexedTuple tup') ?attrlist1%SchemaConstraints ]
-              =>
-              let H' := fresh in
-              generalize (@refine_unused_key_check h attrlist1 attrlist2 _ _ n (qs ! R )%QueryImpl) as H'; intros; setoid_rewrite H'; clear H';
-              [ simplify with monad laws |
-                unfold BookStoreListImpl_AbsR in *; split_and; eauto ]
-        | |- context [
-                 forall tup' : @IndexedTuple ?h,
-                   (?qs ! ?R )%QueryImpl tup' ->
-                   tupleAgree (indexedTuple tup') ?n ?attrlist2%SchemaConstraints ->
-                   tupleAgree (indexedTuple tup') ?n  ?attrlist1%SchemaConstraints]
-                =>
-                let H' := fresh in
-                generalize (@refine_unused_key_check' h attrlist1 attrlist2 _ _ n (qs ! R )%QueryImpl) as H'; intros; setoid_rewrite H'; clear H';
-                  [ simplify with monad laws |
-                    unfold BookStoreListImpl_AbsR in *; split_and; eauto ]
-      end.
-      rewrite refine_pick_eq_ex_bind; unfold BookStoreListImpl_AbsR in *.
-      split_and; simpl;
-      rewrite refineEquiv_pick_pair_pair;
-      setoid_rewrite refineEquiv_pick_eq';
-      simplify with monad laws; simpl.
-      Split Constraint Checks.
-      (* TODO move this back to a tactic *)
-      subst_strings; setoid_rewrite (@ImplementListInsert_eq); eauto.
-      simplify with monad laws.
-      match goal with
-          |- context
-               [{a | EnsembleIndexedListEquivalence
-                       ((@UpdateUnConstrRelation ?QSSchema ?c ?Ridx
-                                                (EnsembleInsert ?n (?c!?R)))!?R')%QueryImpl a}%comp] =>
-          let H := fresh in
-          generalize ((@ImplementListInsert_neq QSSchema
-                                                {| bindex := R' |}
-                                                {| bindex := R |} n c)) as H; intros; setoid_rewrite H
-      end; try reflexivity; try eassumption.
-      congruence.
-      rewrite refine_pick_val; eauto;
-      simplify with monad laws.
-      rewrite refine_pick_val; eauto;
-      simplify with monad laws.
+      (*setoid_rewrite (fun c => where''' _ _ c _).*)
+      setoid_rewrite (fun c => where''' a b c (fun b c a => Return c!sISBN a)).
       reflexivity.
-      rewrite refine_pick_val; eauto;
-      simplify with monad laws.
-      rewrite refine_pick_val; eauto;
-      simplify with monad laws.
+ 
+      setoid_rewrite where''''.
       reflexivity.
-      intros.
-      destruct H as [[l l'] _].
-      generalize (l _ H1).
-      unfold not; intros.
-      eapply lt_irrefl.
-      destruct tup; simpl in *; subst.
-      eapply H.
-    }
 
-    hone method "GetTitles".
-    {
-      simpl.
-      unfold BookStoreListImpl_AbsR in H; split_and.
-      setoid_rewrite refineEquiv_pick_ex_computes_to_and.
-      simplify with monad laws.
-      rewrite refine_List_Query_In; eauto.
-      subst_strings; rewrite refine_List_Query_In_Where.
-      rewrite refine_List_For_Query_In_Return;
-        simplify with monad laws; simpl.
+      setoid_rewrite H2.
+      unfold decider.
 
-      setoid_rewrite refineEquiv_pick_pair_pair.
-      setoid_rewrite refineEquiv_pick_eq'.
+      apply refine_Query_For.
+
+      setoid_rewrite H4.
+      
+      setoid_rewrite H3.
+        
+      unfold Query_Where.
+      unfold Query_Return.
+      pose proof (Equivalent_List_In_Where (A := nat)).
+      clear.
+
+      
+      
+
+      admit.
+
+      rewrite H2.
+
+      (* TODO: Why doesn't this rewrite work? *)      
+
+      pose proof  (fun (a: Book) => Equivalent_UnConstr_In_EnsembleListEquivalence c _ (fun tup0 : Order =>
+                      Where (a!sISBN = tup0!sISBN)
+                      Return tup0!sISBN) H1).
+
+
+
+
+
+Add Parametric Morphism {A: Type} {h1: Heading}
+    qsSchema qs R P
+:
+  (fun (bod: Tuple -> Tuple -> Ensemble A) => Query_For (fun a => exists (b: @Tuple h1), (P b) /\ @UnConstrQuery_In qsSchema qs A R (bod b) a))
+    with signature ((pointwise2_relation (@Tuple h1) (@Tuple _) (@Equivalent_Ensembles A) ==> refine ))
+      as refine_Query_For_In_Equivalent.
+Proof.
+  admit.
+Qed.
+
+
+
+Add Parametric Morphism {A: Type} {h1: Heading}
+     P
+:
+  (fun (Q: Tuple -> Ensemble A) => Query_For (fun a => exists (b: @Tuple h1), (P b) /\ (Q b a)))
+    with signature ((pointwise_relation (@Tuple _) (@Equivalent_Ensembles A) ==> refine ))
+      as refine_Query_For_In_Equivalent'.
+Proof.
+  admit.
+Qed.
+
+Show.
+
+assert (forall {A qsSchema} heading c orders f, pointwise_relation (@Tuple heading) Equivalent_Ensembles
+                                            (fun b => fun a => UnConstrQuery_In (A := A) (qsSchema := qsSchema) c orders (f b) a)
+                                            (fun b => fun a => True)) by (clear; admit).
+
+Typeclasses eauto := debug. (* 5 *)
+
+pose proof (H3 nat _ _ c Orders (fun (b: @Tuple
+               (schemaHeading
+                  (relSchema
+                     (@nth_Bounded NamedSchema string relName
+                        (qschemaSchemas BookStoreSchema) Books)))) tup => Where (b!sISBN = tup!sISBN)
+        Return tup!sISBN)).
+
+(*Focus 2.*)
+
+About refine_Query_For_In_Equivalent'.
+set (a := benumerate (fst r_n)).
+rewrite refine_Query_For_In_Equivalent.
+rewrite (refine_Query_For_In_Equivalent' (fun b => List.In b (filter dec a)) H4).
+
+
+
+setoid_rewrite H4.
+
+      setoid_rewrite H2.  (fun a => Equivalent_UnConstr_In_EnsembleListEquivalence).
+
+ 
+rewrite H2.
+
+      assert (
+          forall aa,
+            Equivalent_Ensembles
+              (UnConstrQuery_In c (BookStoreSchema / sORDERS)
+                                (fun tup0 : Order =>
+                                   Where (aa = tup0!sISBN)
+                                         Return tup0!sISBN ))
+              (fun
+                  a : _ =>
+                  exists tup : Tuple,
+                    List.In tup (benumerate (snd r_n)) /\
+                    (fun tup0 : Order =>
+                       Where (aa = tup0!sISBN)
+                             Return tup0!sISBN ) tup a)).
+      clear H0; admit.
+
+       setoid_rewrite H2.
+
+      rewrite (filter_by_equiv _ (bfind_matcher (Bag := BagProof BookStorage) (Some n, (None, [])))) by (clear; admit).
+
+      setoid_rewrite (bfind_correct _).
+      assert (forall a b, a/\ b <-> b /\ a) as sym by (clear H0; admit).
+*)
+      About Equivalent_Join_Lists.
+      
+ 
+      Lemma Equivalent_Join_Lists' :
+        forall (A B : Type) (qsSchema : QueryStructureSchema)
+               (qs : UnConstrQueryStructure qsSchema) (R : BoundedString) 
+               (l : list B) (l' : list Tuple) (bod : B -> Tuple -> Ensemble A),
+          EnsembleListEquivalence (GetUnConstrRelation qs R) l' ->
+          Equivalent_Ensembles
+            (fun a : A => exists b : B, List.In b l /\ UnConstrQuery_In qs R (bod b) a)
+            (fun a : A =>
+               exists b : B * Tuple, List.In b (Join_Lists l l') /\ bod (fst b) (snd b) a).
+        admit.
+      Qed.
+      
+      rewrite Equivalent_Join_Lists by eassumption.
+
+
+      assert (forall {A} (seq: list (list A)), SetEq (fold_left (@app A) seq []) (flatten seq)) by (clear; admit).
+
+      assert (
+          Equivalent_Ensembles
+            (fun a : nat =>
+               exists b : Book * Order,
+                 List.In b
+                         (Join_Lists (bfind (fst r_n) (Some n, (None, [])))
+                                     (benumerate (snd r_n))) /\
+                 Where ((fst b)!sISBN = (snd b)!sISBN)
+                       Return (snd b)!sISBN  a)
+            (fun a => 
+               exists b : Book * Order,
+                 let snd_db := (benumerate (snd r_n)) in
+                 List.In b
+                         (flatten
+                            (map
+                               (fun a0 : Book =>
+                                  map (fun b0 : Order => (a0, b0)) (filter (fun (b0: Order) => beq_nat a0!sISBN b0!sISBN) snd_db)
+                               )
+                               (bfind (fst r_n) (Some n, (None, []))))) /\
+                         Return (snd b)!sISBN  a)
+        ).
+      clear; admit.
+
+
+      setoid_rewrite H3.
+
+      clear sym H2 H3.
+      Check filter_by_equiv.
+      rewrite (filter_by_equiv _ (bfind_matcher (Bag := BagProof OrderStorage) (Some _, []))). by (clear; admit).
+
+
+      unfold Join_Lists.
+      setoid_rewrite H2.
+
+
+      setoid_rewrite H2.
+      setoid_rewrite in_flatten_iff.
+      setoid_rewrite in_map_iff.
+      rewrite flatten_filter.
+
+      unfold Join_Lists.
+Show.
+      
+      
+      setoid_rewrite Equivalent_List_In_Where.
+      unfold Join_Lists.
+
+      unfold dec. unfold DecideableEnsemble_EqDec.
+
+      rewrite (filter_by_equiv _ (bfind_matcher (Bag := BagProof BookStorage) (Some n, (None, [])))) by (clear; admit).
+
+      SearchAbout filter flatten.
+
+      rewrite filter
+
+      rewrite (filter_by_equiv _ (bfind_matcher (Bag := BagProof BookStorage) (Some n, (None, [])))) by (clear H0; admit). (* TODO: Handle strings in prove_observational_eq, and use rewrites *)
+
+      setoid_rewrite (bfind_correct _).
+
+
+      setoid_rewrite refine_For_List_Return.
       simplify with monad laws.
-      rewrite refine_pick_val by eassumption.
-      simplify with monad laws.
-      rewrite refine_pick_val by eassumption.
+
+      unfold equivalence.
+      rewrite refine_pick_val by eauto. 
       simplify with monad laws.
       finish honing.
-  }
+    }
+      
 
-    hone method "NumOrders".
-    {
-      simpl.
-      unfold BookStoreListImpl_AbsR in H; split_and.
-      setoid_rewrite refineEquiv_pick_ex_computes_to_and.
-      simplify with monad laws.
-      subst_strings.
-      rewrite refine_List_Query_In; eauto.
-      rewrite refine_Join_List_Query_In; eauto.
-      rewrite refine_List_Query_In_Where.
-      rewrite refine_List_Query_In_Where.
-      rewrite refine_List_For_Query_In_Return;
-        simplify with monad laws; simpl.
 
-      setoid_rewrite refineEquiv_pick_pair_pair.
-      setoid_rewrite refineEquiv_pick_eq'.
-      simplify with monad laws.
-      rewrite refine_pick_val by eassumption.
-      simplify with monad laws.
-      rewrite refine_pick_val by eassumption.
-      simplify with monad laws.
-      finish honing.
-  }
+    (* Step 2: We first swap the order of the 'For's to make the
+         implementation more efficient. *)
 
-    implement_empty_list "InitBookstore" BookStoreListImpl_AbsR.
+
+    (* Step 3: Switch to an implementation of the representation
+       type as a pair of lists of tuples. *)
+
+    implement using lists under BookStoreListImpl_SiR.
+
+    (* Step 4: Profit. :) *)
 
     finish sharpening.
   Defined.
